ed25519: move precomputed table to a static header

code/ed25519/Hacl.Impl.Ed25519.Ladder.fst
@@ -10,7 +10,6 @@ open Lib.Buffer
 open Hacl.Bignum25519
 module F51 = Hacl.Impl.Ed25519.Field51
 
-module LSeq = Lib.Sequence
 module BSeq = Lib.ByteSequence
 
 module LE = Lib.Exponentiation
@@ -18,204 +17,24 @@ module SE = Spec.Exponentiation
 module BE = Hacl.Impl.Exponentiation
 module ME = Hacl.Impl.MultiExponentiation
 module PT = Hacl.Impl.PrecompTable
-module SPT = Hacl.Spec.PrecompBaseTable
-
 module BD = Hacl.Bignum.Definitions
-module BC = Hacl.Bignum.Convert
-module SC = Hacl.Spec.Bignum.Convert
 
 module S = Spec.Ed25519
 
+open Hacl.Impl.Ed25519.PointConstants
+include Hacl.Impl.Ed25519.Group
+include Hacl.Ed25519.PrecompTable
+
 #set-options "--z3rlimit 50 --fuel 0 --ifuel 0"
 
-////////////////////////////////////////////////////
-
-unfold
-let a_spec = S.aff_point_c
-
-unfold
-let refl (a:LSeq.lseq uint64 20{F51.linv a}) : GTot a_spec =
-  S.to_aff_point (F51.refl_ext_point a)
-
-unfold
-let linv_ctx (a:LSeq.lseq uint64 0) : Type0 = True
-
 inline_for_extraction noextract
-let mk_to_ed25519_comm_monoid : BE.to_comm_monoid U64 20ul 0ul = {
-  BE.a_spec = a_spec;
-  BE.comm_monoid = S.mk_ed25519_comm_monoid;
-  BE.linv_ctx = linv_ctx;
-  BE.linv = F51.linv;
-  BE.refl = refl;
-  }
-
-
-inline_for_extraction noextract
-val point_add : BE.lmul_st U64 20ul 0ul mk_to_ed25519_comm_monoid
-let point_add ctx x y xy =
-  let h0 = ST.get () in
-  Spec.Ed25519.Lemmas.to_aff_point_add_lemma
-    (F51.refl_ext_point (as_seq h0 x)) (F51.refl_ext_point (as_seq h0 y));
-  Hacl.Impl.Ed25519.PointAdd.point_add xy x y
-
-
-inline_for_extraction noextract
-val point_double : BE.lsqr_st U64 20ul 0ul mk_to_ed25519_comm_monoid
-let point_double ctx x xx =
-  let h0 = ST.get () in
-  Spec.Ed25519.Lemmas.to_aff_point_double_lemma (F51.refl_ext_point (as_seq h0 x));
-  Hacl.Impl.Ed25519.PointDouble.point_double xx x
-
-
-val make_point_inf:
-  b:lbuffer uint64 20ul ->
-  Stack unit
-  (requires fun h -> live h b)
-  (ensures  fun h0 _ h1 -> modifies (loc b) h0 h1 /\
-    F51.point_inv_t h1 b /\ F51.inv_ext_point (as_seq h1 b) /\
-    S.to_aff_point (F51.point_eval h1 b) == S.aff_point_at_infinity)
-
-let make_point_inf b =
-  let x = getx b in
-  let y = gety b in
-  let z = getz b in
-  let t = gett b in
-  make_zero x;
-  make_one y;
-  make_one z;
-  make_zero t;
-  let h1 = ST.get () in
-  assert (F51.point_eval h1 b == S.point_at_infinity);
-  Spec.Ed25519.Lemmas.to_aff_point_at_infinity_lemma ()
-
-
-inline_for_extraction noextract
-val point_zero : BE.lone_st U64 20ul 0ul mk_to_ed25519_comm_monoid
-let point_zero ctx one = make_point_inf one
-
-
-inline_for_extraction noextract
-let mk_ed25519_concrete_ops : BE.concrete_ops U64 20ul 0ul = {
-  BE.to = mk_to_ed25519_comm_monoid;
-  BE.lone = point_zero;
-  BE.lmul = point_add;
-  BE.lsqr = point_double;
-}
-
-//////////////////////////////////////////////
-
-inline_for_extraction noextract
-val ext_point_to_list: p:S.ext_point_c
-  -> x:list uint64{FStar.List.Tot.length x = 20 /\
-    mk_to_ed25519_comm_monoid.BE.linv (Seq.seq_of_list x)}
-
-let ext_point_to_list p =
-  Hacl.Spec.Ed25519.PrecompTable.ext_point_to_list_lemma p;
-  Hacl.Spec.Ed25519.PrecompTable.ext_point_to_list p
-
-
-val lemma_refl: x:S.ext_point_c ->
-  Lemma (S.mk_ed25519_concrete_ops.SE.to.SE.refl x ==
-    mk_to_ed25519_comm_monoid.BE.refl (Seq.seq_of_list (ext_point_to_list x)))
-
-let lemma_refl x =
-  Hacl.Spec.Ed25519.PrecompTable.ext_point_to_list_eval x
-
-
-inline_for_extraction noextract
-let mk_ed25519_precomp_base_table: SPT.mk_precomp_base_table S.ext_point_c U64 20ul 0ul = {
-  SPT.concr_ops = S.mk_ed25519_concrete_ops;
-  SPT.to_cm = mk_to_ed25519_comm_monoid;
-  SPT.to_list = ext_point_to_list;
-  SPT.lemma_refl = lemma_refl;
-}
-
-inline_for_extraction noextract
-let g_c : S.ext_point_c =
-  Spec.Ed25519.Lemmas.g_is_on_curve ();
-  S.g
-
-unfold let precomp_basepoint_table_list: x:list uint64{FStar.List.Tot.length x = 320} =
-  normalize_term (SPT.precomp_base_table_list mk_ed25519_precomp_base_table g_c 15)
-
-inline_for_extraction noextract
-let precomp_basepoint_table_lseq : LSeq.lseq uint64 320 =
-  normalize_term_spec (SPT.precomp_base_table_list mk_ed25519_precomp_base_table g_c 15);
-  Seq.seq_of_list precomp_basepoint_table_list
-
-
-inline_for_extraction noextract
-let pow_base_point (k:nat) =
-  LE.pow S.mk_ed25519_comm_monoid (S.to_aff_point g_c) k
-
-unfold
-let precomp_table_acc_inv
-  (table_len:nat{table_len * 20 <= max_size_t})
-  (table:LSeq.lseq uint64 (table_len * 20))
-  (j:nat{j < table_len})
-=
-  Math.Lemmas.lemma_mult_lt_right 20 j table_len;
-  Math.Lemmas.lemma_mult_le_right 20 (j + 1) table_len;
-  let bj = LSeq.sub table (j * 20) 20 in
-  F51.linv bj /\ refl bj == pow_base_point j
-
-val precomp_basepoint_table_lemma: unit ->
-  Lemma (forall (i:nat{i < 16}). precomp_table_acc_inv 16 precomp_basepoint_table_lseq i)
-let precomp_basepoint_table_lemma () =
-  normalize_term_spec (SPT.precomp_base_table_list mk_ed25519_precomp_base_table g_c 15);
-  SPT.precomp_base_table_lemma mk_ed25519_precomp_base_table g_c 16 precomp_basepoint_table_lseq
-
-/////////////////////////////////////////////////////
-
-inline_for_extraction noextract
-val make_g: g:point -> Stack unit
-  (requires fun h -> live h g)
-  (ensures fun h0 _ h1 -> modifies (loc g) h0 h1 /\
-    F51.point_inv_t h1 g /\ F51.inv_ext_point (as_seq h1 g) /\
-    F51.point_eval h1 g == S.g)
-
-let make_g g =
-  let gx = getx g in
-  let gy = gety g in
-  let gz = getz g in
-  let gt = gett g in
-
-  [@inline_let] let (x0, x1, x2, x3, x4) =
-    (u64 0x00062d608f25d51a,
-     u64 0x000412a4b4f6592a,
-     u64 0x00075b7171a4b31d,
-     u64 0x0001ff60527118fe,
-     u64 0x000216936d3cd6e5) in
-
-  [@inline_let] let (y0, y1, y2, y3, y4) =
-    (u64 0x0006666666666658,
-     u64 0x0004cccccccccccc,
-     u64 0x0001999999999999,
-     u64 0x0003333333333333,
-     u64 0x0006666666666666) in
-
-  [@inline_let] let (t0, t1, t2, t3, t4) =
-    (u64 0x00068ab3a5b7dda3,
-     u64 0x00000eea2a5eadbb,
-     u64 0x0002af8df483c27e,
-     u64 0x000332b375274732,
-     u64 0x00067875f0fd78b7) in
-
-  make_u64_5 gx x0 x1 x2 x3 x4;
-  make_u64_5 gy y0 y1 y2 y3 y4;
-  make_one gz;
-  make_u64_5 gt t0 t1 t2 t3 t4;
-
-  (**) assert_norm (Spec.Ed25519.g_x ==
-    Hacl.Spec.Curve25519.Field51.Definition.as_nat5 (x0, x1, x2, x3, x4) % Spec.Curve25519.prime);
-  (**) assert_norm (Spec.Ed25519.g_y ==
-    Hacl.Spec.Curve25519.Field51.Definition.as_nat5 (y0, y1, y2, y3, y4) % Spec.Curve25519.prime);
-  (**) assert_norm (Mktuple4?._4 Spec.Ed25519.g ==
-    Hacl.Spec.Curve25519.Field51.Definition.as_nat5 (t0, t1, t2, t3, t4) % Spec.Curve25519.prime);
-  let h1 = ST.get () in
-  assert (F51.point_inv_t h1 g);
-  assert (F51.point_eval h1 g == Spec.Ed25519.g);
-  Spec.Ed25519.Lemmas.g_is_on_curve ()
+let table_inv_w4 : BE.table_inv_t U64 20ul 16ul =
+  [@inline_let] let len = 20ul in
+  [@inline_let] let ctx_len = 0ul in
+  [@inline_let] let k = mk_ed25519_concrete_ops in
+  [@inline_let] let l = 4ul in
+  [@inline_let] let table_len = 16ul in
+  BE.table_inv_precomp len ctx_len k l table_len
 
 
 inline_for_extraction noextract
@@ -253,20 +72,6 @@ let point_mul_noalloc out bscalar q =
     4ul (null uint64) q 4ul 256ul bscalar out
 
 
-val point_mul:
-    out:point
-  -> scalar:lbuffer uint8 32ul
-  -> q:point ->
-  Stack unit
-  (requires fun h ->
-    live h scalar /\ live h q /\ live h out /\
-    disjoint q out /\ disjoint q scalar /\
-    F51.point_inv_t h q /\ F51.inv_ext_point (as_seq h q))
-  (ensures  fun h0 _ h1 -> modifies (loc out) h0 h1 /\
-    F51.point_inv_t h1 out /\ F51.inv_ext_point (as_seq h1 out) /\
-    S.to_aff_point (F51.point_eval h1 out) ==
-    S.to_aff_point (S.point_mul (as_seq h0 scalar) (F51.point_eval h0 q)))
-
 let point_mul out scalar q =
   let h0 = ST.get () in
   SE.exp_fw_lemma S.mk_ed25519_concrete_ops
@@ -276,22 +81,6 @@ let point_mul out scalar q =
   convert_scalar scalar bscalar;
   point_mul_noalloc out bscalar q;
   pop_frame ()
-
-////////////////////////////////////////
-
-inline_for_extraction noextract
-let table_inv : BE.table_inv_t U64 20ul 16ul =
-  [@inline_let] let len = 20ul in
-  [@inline_let] let ctx_len = 0ul in
-  [@inline_let] let k = mk_ed25519_concrete_ops in
-  [@inline_let] let l = 4ul in
-  [@inline_let] let table_len = 16ul in
-  BE.table_inv_precomp len ctx_len k l table_len
-
-
-let precomp_basepoint_table:
-  x:glbuffer uint64 320ul{witnessed x precomp_basepoint_table_lseq /\ recallable x} =
-  createL_global precomp_basepoint_table_list
 
 
 inline_for_extraction noextract
@@ -320,28 +109,17 @@ let point_mul_g_noalloc out bscalar g =
   [@inline_let] let bBits = 256ul in
 
   let h0 = ST.get () in
-  recall_contents precomp_basepoint_table precomp_basepoint_table_lseq;
+  recall_contents precomp_basepoint_table_w4 precomp_basepoint_table_lseq_w4;
   let h1 = ST.get () in
-  precomp_basepoint_table_lemma ();
-  assert (table_inv (as_seq h1 g) (as_seq h1 precomp_basepoint_table));
+  precomp_basepoint_table_lemma_w4 ();
+  assert (table_inv_w4 (as_seq h1 g) (as_seq h1 precomp_basepoint_table_w4));
   assert (F51.point_eval h1 g == g_c);
 
   BE.mk_lexp_fw_table len ctx_len k l table_len
-    table_inv
+    table_inv_w4
     (BE.lprecomp_get_consttime len ctx_len k l table_len)
-    (null uint64) g bLen bBits bscalar (to_const precomp_basepoint_table) out
+    (null uint64) g bLen bBits bscalar (to_const precomp_basepoint_table_w4) out
 
-
-val point_mul_g:
-    out:point
-  -> scalar:lbuffer uint8 32ul ->
-  Stack unit
-  (requires fun h ->
-    live h scalar /\ live h out /\ disjoint out scalar)
-  (ensures  fun h0 _ h1 -> modifies (loc out) h0 h1 /\
-    F51.point_inv_t h1 out /\ F51.inv_ext_point (as_seq h1 out) /\
-    S.to_aff_point (F51.point_eval h1 out) ==
-    S.to_aff_point (S.point_mul_g (as_seq h0 scalar)))
 
 [@CInline]
 let point_mul_g out scalar =
@@ -377,7 +155,7 @@ val point_mul_g_double_vartime_noalloc:
     F51.point_inv_t h q1 /\ F51.inv_ext_point (as_seq h q1) /\
     F51.point_eval h q1 == g_c /\
     F51.point_inv_t h q2 /\ F51.inv_ext_point (as_seq h q2) /\
-    table_inv (as_seq h q2) (as_seq h table2))
+    table_inv_w4 (as_seq h q2) (as_seq h table2))
   (ensures fun h0 _ h1 -> modifies (loc out) h0 h1 /\
     F51.point_inv_t h1 out /\ F51.inv_ext_point (as_seq h1 out) /\
     S.to_aff_point (F51.point_eval h1 out) ==
@@ -395,18 +173,18 @@ let point_mul_g_double_vartime_noalloc out scalar1 q1 scalar2 q2 table2 =
   [@inline_let] let bBits = 256ul in
 
   let h0 = ST.get () in
-  recall_contents precomp_basepoint_table precomp_basepoint_table_lseq;
+  recall_contents precomp_basepoint_table_w4 precomp_basepoint_table_lseq_w4;
   let h1 = ST.get () in
-  precomp_basepoint_table_lemma ();
-  assert (table_inv (as_seq h1 q1) (as_seq h1 precomp_basepoint_table));
-  assert (table_inv (as_seq h1 q2) (as_seq h1 table2));
+  precomp_basepoint_table_lemma_w4 ();
+  assert (table_inv_w4 (as_seq h1 q1) (as_seq h1 precomp_basepoint_table_w4));
+  assert (table_inv_w4 (as_seq h1 q2) (as_seq h1 table2));
 
   ME.mk_lexp_double_fw_tables len ctx_len k l table_len
-    table_inv table_inv
+    table_inv_w4 table_inv_w4
     (BE.lprecomp_get_vartime len ctx_len k l table_len)
     (BE.lprecomp_get_vartime len ctx_len k l table_len)
     (null uint64) q1 bLen bBits scalar1 q2 scalar2
-    (to_const precomp_basepoint_table) (to_const table2) out
+    (to_const precomp_basepoint_table_w4) (to_const table2) out
 
 
 inline_for_extraction noextract
@@ -516,23 +294,6 @@ let point_mul_g_double_vartime out scalar1 scalar2 q2 =
   point_mul_g_double_vartime_aux out scalar1 g scalar2 q2 bscalar1 bscalar2;
   pop_frame ()
 
-
-val point_negate_mul_double_g_vartime:
-    out:point
-  -> scalar1:lbuffer uint8 32ul
-  -> scalar2:lbuffer uint8 32ul
-  -> q2:point ->
-  Stack unit
-  (requires fun h ->
-    live h out /\ live h scalar1 /\
-    live h scalar2 /\ live h q2 /\
-    disjoint q2 out /\ disjoint scalar1 out /\ disjoint scalar2 out /\
-    F51.point_inv_t h q2 /\ F51.inv_ext_point (as_seq h q2))
-  (ensures fun h0 _ h1 -> modifies (loc out) h0 h1 /\
-    F51.point_inv_t h1 out /\ F51.inv_ext_point (as_seq h1 out) /\
-    S.to_aff_point (F51.point_eval h1 out) ==
-    S.to_aff_point (S.point_negate_mul_double_g
-      (as_seq h0 scalar1) (as_seq h0 scalar2) (F51.point_eval h0 q2)))
 
 [@CInline]
 let point_negate_mul_double_g_vartime out scalar1 scalar2 q2 =
