code/ed25519/Hacl.Spec.Ed25519.PrecompTable.fst
@@ -14,61 +14,6 @@ module SPT = Hacl.Spec.PrecompBaseTable
 
 #set-options "--z3rlimit 50 --fuel 0 --ifuel 0"
 
-unfold
-let create5 (x0 x1 x2 x3 x4:uint64) : list uint64 = [x0; x1; x2; x3; x4]
-
-inline_for_extraction noextract
-let felem_list = x:list uint64{FL.length x == 5}
-inline_for_extraction noextract
-let point_list = x:list uint64{FL.length x == 20}
-
-inline_for_extraction noextract
-let pow51 = SF51.pow51
-
-[@"opaque_to_smt"]
-let pow102: (pow102:pos{pow2 102 == pow102 /\ pow102 = pow51 * pow51}) =
-  let pow102:pos = normalize_term (pow2 102) in
-  normalize_term_spec (pow2 102);
-  Math.Lemmas.pow2_plus 51 51;
-  pow102
-
-[@"opaque_to_smt"]
-let pow153: (pow153:pos{pow2 153 == pow153 /\ pow153 = pow51 * pow51 * pow51}) =
-  let pow153:pos = normalize_term (pow2 153) in
-  normalize_term_spec (pow2 153);
-  Math.Lemmas.pow2_plus 51 51;
-  Math.Lemmas.pow2_plus 102 51;
-  pow153
-
-[@"opaque_to_smt"]
-let pow204: (pow204:pos{pow2 204 == pow204 /\ pow204 = pow51 * pow51 * pow51 * pow51}) =
-  let pow204:pos = normalize_term (pow2 204) in
-  normalize_term_spec (pow2 204);
-  Math.Lemmas.pow2_plus 51 51;
-  Math.Lemmas.pow2_plus 102 51;
-  Math.Lemmas.pow2_plus 153 51;
-  pow204
-
-
-inline_for_extraction noextract
-let felem_to_list (x:SC.elem) : felem_list =
-  [@inline_let] let x0 = x % pow51 in
-  [@inline_let] let x1 = x / pow51 % pow51 in
-  [@inline_let] let x2 = x / pow102 % pow51 in
-  [@inline_let] let x3 = x / pow153 % pow51 in
-  [@inline_let] let x4 = x / pow204 in
-  Math.Lemmas.lemma_div_lt_nat x 255 204;
-  [@inline_let] let r = create5 (u64 x0) (u64 x1) (u64 x2) (u64 x3) (u64 x4) in
-  assert_norm (FL.length r = 5);
-  r
-
-
-inline_for_extraction noextract
-let ext_point_to_list (p:S.ext_point) : point_list =
-  [@inline_let] let (px, py, pz, pt) = p in
-  FL.(felem_to_list px @ felem_to_list py @ felem_to_list pz @ felem_to_list pt)
-
-//----------------------------------------------
 
 let create5_lseq (x0 x1 x2 x3 x4:uint64) : lseq uint64 5 =
   let l = [x0; x1; x2; x3; x4] in
@@ -176,18 +121,6 @@ let felem_to_list_lemma_eval x =
 
 //--------------------------------------------
 
-inline_for_extraction noextract
-let point_inv_list (p:point_list) =
-  let x = Seq.seq_of_list p <: lseq uint64 20 in
-  //F51.inv_ext_point x
-  F51.linv x
-
-noextract
-let point_eval_list (p:point_list) : GTot S.ext_point =
-  let x = Seq.seq_of_list p <: lseq uint64 20 in
-  F51.refl_ext_point x
-
-
 val ext_point_to_list_sub: p:S.ext_point -> Lemma
  (let (px, py, pz, pt) = p in
   let px_list = felem_to_list px in
@@ -245,9 +178,6 @@ let ext_point_to_list_eval p =
   Math.Lemmas.small_mod pz SC.prime;
   Math.Lemmas.small_mod pt SC.prime
 
-
-val ext_point_to_list_lemma: p:S.ext_point{Spec.Ed25519.point_inv p} ->
-  Lemma (point_inv_list (ext_point_to_list p) /\ point_eval_list (ext_point_to_list p) == p)
 
 let ext_point_to_list_lemma p =
   ext_point_to_list_eval p;
