code/ed25519/Hacl.Ed25519.PrecompTable.fst
@@ -1,0 +1,106 @@
+module Hacl.Ed25519.PrecompTable
+
+module ST = FStar.HyperStack.ST
+open FStar.HyperStack.All
+open FStar.Mul
+
+open Lib.IntTypes
+open Lib.Buffer
+
+open Hacl.Bignum25519
+module F51 = Hacl.Impl.Ed25519.Field51
+
+module LSeq = Lib.Sequence
+module BSeq = Lib.ByteSequence
+
+module LE = Lib.Exponentiation
+module SE = Spec.Exponentiation
+module BE = Hacl.Impl.Exponentiation
+module ME = Hacl.Impl.MultiExponentiation
+module PT = Hacl.Impl.PrecompTable
+module SPT = Hacl.Spec.PrecompBaseTable
+
+module BD = Hacl.Bignum.Definitions
+module BC = Hacl.Bignum.Convert
+module SC = Hacl.Spec.Bignum.Convert
+
+module S = Spec.Ed25519
+
+open Hacl.Impl.Ed25519.PointConstants
+include Hacl.Impl.Ed25519.Group
+
+#set-options "--z3rlimit 50 --fuel 0 --ifuel 0"
+
+inline_for_extraction noextract
+val ext_point_to_list: p:S.ext_point_c
+  -> x:list uint64{FStar.List.Tot.length x = 20 /\
+    mk_to_ed25519_comm_monoid.BE.linv (Seq.seq_of_list x)}
+
+let ext_point_to_list p =
+  Hacl.Spec.Ed25519.PrecompTable.ext_point_to_list_lemma p;
+  Hacl.Spec.Ed25519.PrecompTable.ext_point_to_list p
+
+
+val lemma_refl: x:S.ext_point_c ->
+  Lemma (S.mk_ed25519_concrete_ops.SE.to.SE.refl x ==
+    mk_to_ed25519_comm_monoid.BE.refl (Seq.seq_of_list (ext_point_to_list x)))
+
+let lemma_refl x =
+  Hacl.Spec.Ed25519.PrecompTable.ext_point_to_list_lemma x
+
+
+inline_for_extraction noextract
+let mk_ed25519_precomp_base_table: SPT.mk_precomp_base_table S.ext_point_c U64 20ul 0ul = {
+  SPT.concr_ops = S.mk_ed25519_concrete_ops;
+  SPT.to_cm = mk_to_ed25519_comm_monoid;
+  SPT.to_list = ext_point_to_list;
+  SPT.lemma_refl = lemma_refl;
+}
+
+
+inline_for_extraction noextract
+let g_c : S.ext_point_c =
+  Spec.Ed25519.Lemmas.g_is_on_curve ();
+  S.g
+
+
+inline_for_extraction noextract
+let pow_base_point (k:nat) =
+  LE.pow S.mk_ed25519_comm_monoid (S.to_aff_point g_c) k
+
+unfold
+let precomp_table_acc_inv
+  (table_len:nat{table_len * 20 <= max_size_t})
+  (table:LSeq.lseq uint64 (table_len * 20))
+  (j:nat{j < table_len})
+=
+  Math.Lemmas.lemma_mult_lt_right 20 j table_len;
+  Math.Lemmas.lemma_mult_le_right 20 (j + 1) table_len;
+  let bj = LSeq.sub table (j * 20) 20 in
+  F51.linv bj /\ refl bj == pow_base_point j
+
+
+///  window size = 4
+
+unfold let precomp_basepoint_table_list_w4: x:list uint64{FStar.List.Tot.length x = 320} =
+  normalize_term (SPT.precomp_base_table_list mk_ed25519_precomp_base_table g_c 15)
+
+
+inline_for_extraction noextract
+let precomp_basepoint_table_lseq_w4 : LSeq.lseq uint64 320 =
+  normalize_term_spec (SPT.precomp_base_table_list mk_ed25519_precomp_base_table g_c 15);
+  Seq.seq_of_list precomp_basepoint_table_list_w4
+
+
+val precomp_basepoint_table_lemma_w4: unit ->
+  Lemma (forall (i:nat{i < 16}). precomp_table_acc_inv 16 precomp_basepoint_table_lseq_w4 i)
+
+let precomp_basepoint_table_lemma_w4 () =
+  normalize_term_spec (SPT.precomp_base_table_list mk_ed25519_precomp_base_table g_c 15);
+  SPT.precomp_base_table_lemma
+    mk_ed25519_precomp_base_table g_c 16 precomp_basepoint_table_lseq_w4
+
+
+let precomp_basepoint_table_w4:
+  x:glbuffer uint64 320ul{witnessed x precomp_basepoint_table_lseq_w4 /\ recallable x} =
+  createL_global precomp_basepoint_table_list_w4
